cedar-lean/Cedar/Thm/Data/Control.lean
@@ -80,7 +80,7 @@ theorem to_option_none {res: Except ε α} :
   rename_i err
   exists err
 
-theorem to_option_left_ok {v : α} {res₁ res₂ : Except ε α} :
+theorem to_option_left_ok {α ε₁ ε₂} {v : α} {res₁ : Except ε₁ α} {res₂ : Except ε₂ α} :
   res₁.toOption = res₂.toOption → res₁ = .ok v → res₂ = .ok v
 := by
   intro h₀ h₁
@@ -93,14 +93,29 @@ theorem to_option_left_ok {v : α} {res₁ res₂ : Except ε α} :
   · cases h₀
   · cases h₁
 
-theorem to_option_right_ok {v : α} {res₁ res₂ : Except ε α} :
+theorem to_option_right_ok {α ε₁ ε₂} {v : α} {res₁ : Except ε₁ α} {res₂ : Except ε₂ α} :
   res₁.toOption = res₂.toOption → res₂ = .ok v → res₁ = .ok v
 := by
   intro h
   symm at h
   exact to_option_left_ok h
 
-theorem to_option_left_err {err₁: ε} {res₂ : Except ε α} :
+theorem to_option_right_ok' {α ε₁ ε₂} {v : α} {res₁ : Except ε₁ α} :
+  res₁.toOption = ((.ok v) : Except ε₂ α).toOption → res₁ = Except.ok v
+:= by
+  generalize h : ((.ok v) : Except ε₂ α) = res₂
+  symm at h
+  intro h₁
+  exact to_option_right_ok h₁ h
+
+theorem to_option_left_ok' {α ε₁ ε₂} {v : α} {res₂ : Except ε₂ α} :
+  ((.ok v) : Except ε₁ α).toOption = res₂.toOption → res₂ = Except.ok v
+:= by
+  intro h
+  symm at h
+  exact to_option_right_ok' h
+
+theorem to_option_left_err {ε₁ ε₂ α} {err₁: ε₁} {res₂ : Except ε₂ α} :
   (Except.error err₁).toOption = res₂.toOption → ∃ err₂, res₂ = .error err₂
 := by
   intro h
@@ -109,7 +124,7 @@ theorem to_option_left_err {err₁: ε} {res₂ : Except ε α} :
   · cases h
   · simp only [Except.error.injEq, exists_eq']
 
-theorem to_option_right_err {err₂: ε} {res₁ : Except ε α} :
+theorem to_option_right_err {ε₂ ε₁ α} {err₂: ε₂} {res₁ : Except ε₁ α} :
   res₁.toOption = (Except.error err₂).toOption → ∃ err₁, res₁ = .error err₁
 := by
   intro h
